lean/STLC/STLC.lean
@@ -1,3 +1,6 @@
 -- This module serves as the root of the `STLC` library.
 -- Import modules here that should be built as part of the library.
-import STLC.Basic
+
+import STLC.Smallstep
+import STLC.Smallstep_Ctx
+import STLC.Smallstep_LR
