lean/STLC/STLC/Env.lean
@@ -1,0 +1,29 @@
+import Mathlib.Data.Finset.Sort
+
+@[simp]
+def indexr {X : Type} (n : ℕ) (l : List X) : Option X :=
+  match l with
+  | [] => none
+  | a :: l' => if n == l'.length then some a else indexr n l'
+
+lemma indexrSome : ∀ {A} (xs : List A) i,
+  i < xs.length -> ∃ x, indexr i xs = some x := by
+  intro A xs i h; induction xs
+  case nil => simp at h
+  case cons x xs ih =>
+    simp; by_cases h': i = xs.length
+    . simp [h']
+    . simp [if_neg h']; apply ih; simp at h; omega
+
+lemma indexrSome' : ∀ {A} (xs : List A) i,
+  (∃ x, indexr i xs = some x) → i < xs.length := by
+  intros A xs i h; induction xs
+  case nil => simp at h
+  case cons x xs ih =>
+    simp at h; by_cases h': i = xs.length
+    . subst h'; simp
+    . simp [if_neg h'] at h; simp;
+      have h' := ih h; omega
+
+lemma indexrHead : ∀ {A} (x : A) (xs : List A),
+  indexr xs.length (x :: xs) = some x := by intros A x xs; simp
